ok
git-svn-id: svn://scm.gforge.inria.fr/svn/cfml@211 ba02c806-7d2b-4818-9a48-35b22e6bdc79

ImpCF.v
@@ -184,20 +184,20 @@ Definition cf_skip : Formula :=
   weaken (fun H Q => H ===> Q).
 
 Definition cf_ass (V : id) (a : aexp) : Formula :=
-  fun H Q => H ===> (fun st => Q (update st V (aeval st a))).
+  weaken (fun H Q => H ===> (fun st => Q (update st V (aeval st a)))).
 
 Definition cf_seq (F1 F2 : Formula) : Formula :=
-  fun H Q => exists H', F1 H H' /\ F2 H' Q.
+  weaken (fun H Q => exists H', F1 H H' /\ F2 H' Q).
 
 Definition cf_if (b : bexp) (F1 F2 : Formula) : Formula :=
-  fun H Q => F1 (fun st => H st /\ bassn b st) Q
-          /\ F2 (fun st => H st /\ ~ bassn b st) Q.
+  weaken (fun H Q => F1 (fun st => H st /\ bassn b st) Q
+                  /\ F2 (fun st => H st /\ ~ bassn b st) Q).
 
 Definition cf_while (b : bexp) (F1 : Formula) : Formula :=
-  fun H Q => forall (R:Formula),
+  weaken (fun H Q => forall (R:Formula),
     (forall H' Q',
       (cf_if b (cf_seq F1 R) cf_skip) H' Q' -> R H' Q') ->
-    R H Q.
+    R H Q).
 
 Notation "'\SKIP'" := 
   cf_skip.
@@ -237,49 +237,43 @@ Lemma beval_false : forall st b,
 Proof. intros. unfold bassn. rewrite~ H. Qed. 
 Hint Resolve beval_false.
 
+Definition sound (c:com) (R:Formula) :=
+  forall P Q, R P Q -> forall st, P st ->
+    exists st', c / st ==> st' /\ Q st'.
 
-Lemma cf_sound : forall (c:com) (P Q:Assertion), 
-  cf c P Q -> forall st, P st -> exists st', c / st ==> st' /\ Q st'.
+Lemma sound_weaken : forall c R,
+  sound c R -> sound c (weaken R).
 Proof.
-  induction c; intros P Q H st Hst.
-  unfolds in H. unfolds in H.
-  specializes H Hst. destruct H as (P'&Q'&Pre&Main&Post).
+  introv M Wea Pre.
+  destruct (Wea _ Pre) as (P'&Q'&Pre'&Main&Post').
+  forwards* (st'&?&?): M. 
+Qed.
 
-  
+Lemma cf_sound : forall (c:com), sound c (cf c).
+Proof.
+  induction c; simpl; apply sound_weaken; intros H Q F st Hst.
   eauto.
-  eauto.
-  destruct H as (H'&H1&H2).
+  eauto. 
+  destruct F as (H'&H1&H2).
    forwards* (st1&Red1&Post1): (>>> IHc1 H1).
    forwards* (st2&Red2&Post2): (>>> IHc2 H2).
-  destruct H as (H1&H2). case_eq (beval st b); intro B.
+  destruct F as (H1&H2). case_eq (beval st b); intro B.
    forwards* (st1&Red1&Post1): (>>> IHc1 H1).
    forwards* (st2&Red2&Post2): (>>> IHc2 H2).
-  gen st. pattern P. pattern Q. apply H.
-   clear H Q. intros H Q [M1 M2] st Hst.
+  gen st. apply F. clear F H Q. intros H Q M st Hst.
+   destruct (M _ Hst) as (H'&Q'&Pre'&(M1&M2)&Post'). clear M.
    case_eq (beval st b); intro B.
-     destruct M1 as (H'&M11&M12).
+     forwards~ (P''&Q''&?&(H''&M11&M12)&?): (M1 st). clear M1 M2.
       forwards* (st1&Red1&Post1): (>>> IHc M11).
       forwards* (st2&Red2&Post2): M12.
-     hnf in M2. eauto 7.
+      esplit. split. apply* E_WhileLoop. eauto.
+     forwards* (?&?&?&?&?): (M2 st). eauto 8.
 Qed.
 
 
-Lemma cf_sound : forall (c:com) (P Q:Assertion), 
-  cf c P Q -> forall st, P st -> exists st', c / st ==> st' /\ Q st'.
-
-(*****************************************************************************)
-(** Completeness proof *)
-
-Lemma cf_complete : forall (c:com) (st st':state), 
-  c / st ==> st'  ->  cf c (= st) (= st').
-Proof.
-  introv H. induction H.
-  hnf. simple~.
-  hnf. simpl. intros. subst~.
-  hnf. exists~ (=st').
-  hnf. split.
-  
-Qed.
+Lemma cf_sound' : forall (c:com) (P Q:Assertion) (st:state), 
+  cf c P Q -> P st -> exists st', c / st ==> st' /\ Q st'.
+Proof. intros. apply* cf_sound. Qed.
 
 
 (*****************************************************************************)
@@ -308,4 +302,269 @@ Proof.
   forwards* E: (>>> deterministic Red Red').
   rewrite~ E.
 Qed.
+
+(********************************************************************)
+(* ** Facto *)
+
+Module Factorial.
+
+Fixpoint real_fact (n:nat) : nat :=
+  match n with
+  | O => 1
+  | S n' => n * (real_fact n')
+  end.
+
+Definition fact_body : com :=
+  Y ::= AMult (AId Y) (AId Z);
+  Z ::= AMinus (AId Z) (ANum 1).
+
+Definition fact_loop : com :=
+  WHILE BNot (BEq (AId Z) (ANum 0)) DO
+    fact_body
+  END.
+
+Definition fact_com : com :=
+  Z ::= (AId X);
+  Y ::= ANum 1;
+  fact_loop.
+
+Tactic Notation "xseq" :=
+  hnf; eapply weaken_elim; esplit; split.
+Tactic Notation "xseq" constr(H) :=
+  hnf; eapply weaken_elim; exists H; split.
+
+Axiom beq_id_refl : forall x, beq_id x x = true.
+
+Lemma assignement : forall st V X,
+  update st V (aeval st (AId X)) V = st X.
+Proof.
+  intros. unfold aeval, update. rewrite~ beq_id_refl.
+Qed.
+
+Lemma ass_eq : forall st V a,
+  update st V a V = a.
+Proof.
+  intros. unfold aeval, update. rewrite~ beq_id_refl.
+Qed.
+
+Lemma ass_neq : forall st V V' a,
+  V <> V' ->
+  update st V a V' = st V'.
+Proof.
+  intros. unfold aeval, update. skip. (* todo *)
+Qed.
+
+Tactic Notation "xass" :=
+  let st := fresh "st" in let Pst := fresh "Pst" in
+  hnf; eapply weaken_elim; intros st Pst;
+  repeat rewrite ass_eq; repeat rewrite ass_neq;
+  simpl aeval.
+  (*try rewrite assignement.*)
+
+Tactic Notation "xwhile" :=
+  let R := fresh "R" in let HR := fresh "H" R in
+  hnf; eapply weaken_elim; intros R HR.
+
+Tactic Notation "xif" :=
+  hnf; eapply weaken_elim; split.
+
+Lemma mult_one : forall x, x = 1 * x.
+Proof. intros. simpl. apply plus_n_O. Qed.
+
+(*Require LibNat.*)
+Axiom peano_induction : forall P : nat -> Prop,
+   (forall n : nat, (forall m : nat, lt m n -> P m) -> P n) ->
+ forall n : nat, P n.
+
+Tactic Notation "xskip" :=
+  let st := fresh "st" in let Pst := fresh "Pst" in
+  hnf; eapply weaken_elim; intros st Pst.
+
+Lemma end_loop : forall Z st,
+  ~ bassn (BNot (BEq (AId Z) (ANum 0))) st -> st Z = 0.
+Proof.
+  intros. simpls. unfolds bassn, beval. simpls.
+  destruct (st Z0); simpls. auto. false. 
+Qed.
+Require Arith Omega.
+
+Hint Extern 1 (Y <> Z) => skip.
+Hint Extern 1 (Z <> Y) => skip.
+
+Theorem fact_com_correct : forall x,
+  cf fact_com (fun st => st X = x)
+              (fun st => st Y = real_fact x).
+Proof.
+  intros x. 
+  xseq (fun st => st Z = x). xass. auto.
+  xseq (fun st => st Z = x /\ st Y = 1). xass; auto. 
+  xwhile. cuts M: (forall n k, 
+    R (fun st => st Z = n /\ st Y = k)
+      (fun st => st Y = k * real_fact n)).
+    rewrite (mult_one (real_fact x)). apply M.
+   induction n using peano_induction; intros k.
+   apply HR. xif.
+     asserts: (n <> 0). skip. destruct n as [|n']. false.
+     xseq (fun st => st Z = n' /\ st Y = k * (S n')).     
+       xseq (fun st => st Z = S n' /\ st Y = k * (S n')).
+         xass; auto*.
+         xass; auto. destruct Pst. omega.
+       unfold real_fact. fold (real_fact n').
+        rewrite Mult.mult_assoc. apply~ H.
+     xskip. destruct Pst as [[I J] K]. rewrite J.
+      lets: (end_loop K). asserts_rewrite (n = 0). omega.
+      simpl. omega.
+End Factorial.
+
+
+
+
+(********************************************************************)
+(* ** Tactics *)
+
+Ltac xcf :=
+  intros; apply cf_sound; simpl.
+
+Ltac xdone := 
+  hnf.
+
+Ltac xseq :=
+  esplit; split.
+
+Ltac xwrite :=
+  hnf; simpl; try reflexivity.
+
+Ltac xwhile P I W X0 :=
+  esplit; exists P; exists I; exists W; 
+  split; [|split; [exists X0; split|]].
+
+
+Fixpoint fact (n:nat) : nat :=
+  match n with
+  | 0 => 1
+  | S n' => n * (fact n')
+  end.
+
+Fixpoint prod_from (n:nat) (k:nat) : nat :=
+  match k with
+  | 0 => 1
+  | S k' => n * prod_from (S n) k'
+  end.
+
+Lemma prod_from_cut : forall m n, m <= n ->
+  fact (n-m) * prod_from (S(n-m)) m = fact n.
+Proof.
+  intros m n. induction m; intros Le.
+  simpl. math_rewrite (n-0=n). omega.
+  rewrite <- IHm; try omega.
+  simpl. math_rewrite (n-m=S(n-(S m))). simpl. ring.
+Qed.
+
+Lemma prod_from_zero : forall n, n > 0 ->
+  prod_from 1 n = fact n.
+Proof.
+  intros. destruct n. omega.
+  rewrite <- (prod_from_cut n); try omega.
+  math_rewrite (S n - n = 1). simpl. auto.
+Qed.
+
+Lemma prod_from_succ : forall i k,
+  prod_from i (S k) = i * prod_from (S i) k.
+Proof. auto. Qed.
+
+(********************************************************************)
+(* ** Facto verif *)
+
+
+Lemma facto_proof' : forall n, n > 0 ->
+  red facto '[N := n; M := 1] '[N := 0; M := fact n].
+Proof.
+  xcf.
+  xwhile (fun i => i <= n)
+         (fun i => '[N:=i; M:=prod_from (S i) (n-i)])
+         lt 
+         n.  
+  apply lt_wf.
+  omega. 
+  repeat fequal. math_rewrite (n-n=0). auto.
+  (* loop *)
+  simpl. intros i Le. destruct (i == 0).
+    subst i. rewrite prod_from_zero; math_fequal. 
+    exists (i-1). split; [|split]; try omega.
+  (* body of the loop *)
+  xseq.
+  xwrite.
+  xwrite. rewrite <- prod_from_succ. math_fequal.
+Qed.
+
+
+
+
+(*****************************************************************************)
+(** Completeness proof *)
+
+Ltac introeq := 
+  let x := fresh in intros x; intro; subst x.
+
+Lemma assertion_impl_trans : forall H2 H1 H3,
+  H1 ===> H2 -> H2 ===> H3 -> H1 ===> H3.
+Proof. intros_all~. Qed.
+
+Lemma weaken_idem : forall (R:Formula) H Q,
+  weaken (weaken R) H Q -> weaken R H Q.
+Proof.
+  introv M Pre. destruct~ (M st) as (H'&Q'&?&?&I1).
+  destruct~ (H1 st) as (H''&Q''&?&?&I2).
+  lets*: (>>> assertion_impl_trans I2 I1).
+Qed.
+
+Lemma weaken_cf : forall (c:com) (H Q : Assertion),
+  weaken (cf c) H Q -> cf c H Q.
+Proof. intros. destruct c; apply~ weaken_idem. Qed.
+ 
+Lemma cf_name : forall (c:com) (H Q : Assertion),
+  (forall st, H st -> cf c (= st) Q) -> cf c H Q. 
+Proof. intros. apply weaken_cf. apply~ weaken_name. Qed.
+
+
+Lemma cf_complete : forall (c:com) (st st':state), 
+  c / st ==> st'  ->  cf c (= st) (= st'). 
+Proof.
+  introv H. induction H; simpl.
+  apply~ weaken_elim.
+  apply~ weaken_elim. introeq. subst~.
+  apply~ weaken_elim. exists~ (=st').
+  apply~ weaken_elim. split.
+    eapply cf_name. intros st2 [? ?]. subst~.
+    eapply cf_name. intros st2 [? G]. subst. false*.
+  apply~ weaken_elim. split.
+    eapply cf_name. intros st2 [? G]. subst. false*.
+    eapply cf_name. intros st2 [? ?]. subst~.
+  apply~ weaken_elim. intros R M.
+    apply M. clear M. apply weaken_elim. split.
+      eapply weaken_name. intros st2 [? ?]. subst. false*.
+      eapply weaken_name. intros st2 [? G]. subst~.
+  apply~ weaken_elim. intros R M.
+    asserts* F: ((WHILE b1 DO c1 END) / st ==> st'').
+    clear H H0 H1 IHceval1 IHceval2. 
+    gen_eq E: (WHILE b1 DO c1 END).
+    gen_eq S1: st.
+    gen_eq S1': st'. gen st st'.
+    induction F; intros; subst; tryfalse.
+    skip.
+    inversions H2.
+    apply M. apply weaken_elim. split. 
+      eapply weaken_name. intros st2 [? ?]. subst. 
+       exists (=st'). split~. skip.
+      eapply weaken_name. intros st2 [? G]. subst. false*.
+    
+    
+
+
+    apply M. clear M. apply weaken_elim. split.
+      eapply weaken_name. intros st2 [? ?]. subst. 
+       exists (=st'). split~. skip.
+      eapply weaken_name. intros st2 [? G]. subst. false*.
+Qed.
+
 
